Infra/MoreList.v
@@ -651,3 +651,14 @@ Instance zip_eq_m (X Y Z : Type)
 Proof.
   unfold Proper, respectful; intros; subst; eauto.
 Qed.
+
+Lemma fold_list_length A B (f:list B -> (list A * bool) -> list B) (a:list (list A * bool)) (b: list B)
+  : (forall n aa, get a n aa -> ❬b❭ <= ❬fst aa❭)
+    -> (forall aa b, ❬b❭ <= ❬fst aa❭ -> ❬f b aa❭ = ❬b❭)
+    -> length (fold_left f a b) = ❬b❭.
+Proof.
+  intros LEN.
+  general induction a; simpl; eauto.
+  erewrite IHa; eauto 10 using get with len.
+  intros. rewrite H; eauto using get.
+Qed.
