UnreachableCodeAnalysisCorrect.v
@@ -1,0 +1,142 @@
+Require Import CSet Le Var.
+
+Require Import Plus Util AllInRel Map CSet OptionR.
+Require Import Val Var Env EnvTy IL Annotation Lattice DecSolve Analysis Filter Terminating.
+Require Import Analysis AnalysisForward UnreachableCodeAnalysis UnreachableCode Subterm.
+
+Set Implicit Arguments.
+
+Lemma forward_getAnn (sT:stmt) (Dom : stmt -> Type) `{BoundedSemiLattice (Dom sT)}
+      (f: forall sT, list params ->
+                forall s, subTerm s sT -> Dom sT -> anni (Dom sT)) s (ST:subTerm s sT) ZL a an
+  : ann_R eq (fst (@forward sT Dom _ _ f ZL s ST (setTopAnn an a))) an
+    -> getAnn an = a.
+Proof.
+  intros. destruct s, an; inv H1; simpl in *; eauto;
+  repeat let_case_eq; repeat simpl_pair_eqs; subst; simpl in *; inv H2; eauto.
+Qed.
+
+Lemma setTopAnn_eta A (an:ann A) a
+  : getAnn an = a
+    -> setTopAnn an a = an.
+Proof.
+  intros; destruct an; simpl in *; subst; eauto.
+Qed.
+
+Local Arguments proj1_sig {A} {P} e.
+Local Arguments length {A} e.
+Local Arguments forward {sT} {Dom} {H} {H0} ftransform ZL st ST a.
+
+Ltac simpl_forward_setTopAnn :=
+  repeat match goal with
+         | [H : ann_R eq (fst (forward ?unreachable_code_transform ?ZL ?s ?ST (setTopAnn ?sa ?a))) ?sa |- _ ] =>
+           let X := fresh "H" in
+           match goal with
+           | [ H' : getAnn sa = a |- _ ] => fail 1
+           | _ => exploit (forward_getAnn _ _ _ _ _ H) as X
+           end
+         end; rewrite setTopAnn_eta in *; try eassumption.
+
+Lemma PIR2_fstNoneOrR_inv_left A B C
+  : PIR2 (fstNoneOrR impb) (ojoin bool orb ⊜ A B) C
+    -> length A = length B
+    -> PIR2 (fstNoneOrR impb) A C.
+Proof.
+  intros. length_equify.
+  general induction H; inv H0; simpl in *; eauto using PIR2; try solve [ congruence ].
+  - inv Heql; econstructor; eauto.
+    + inv Heql.
+      destruct x0, y0; simpl in *; inv pf; econstructor; eauto.
+      destruct b, b0, y0; simpl in *; eauto.
+Qed.
+
+Lemma PIR2_fstNoneOrR_inv_right A B C
+  : PIR2 (fstNoneOrR impb) (ojoin bool orb ⊜ A B) C
+    -> length A = length B
+    -> PIR2 (fstNoneOrR impb) B C.
+Proof.
+  intros. length_equify.
+  general induction H; inv H0; simpl in *; eauto using PIR2; try solve [ congruence ].
+  - inv Heql; econstructor; eauto.
+    + inv Heql.
+      destruct x0, y0; simpl in *; inv pf; econstructor; eauto.
+      destruct b, b0, y0; simpl in *; eauto.
+Qed.
+
+Definition unreachable_code_analysis_correct sT ZL BL s a (ST:subTerm s sT)
+  : ann_R poEq (fst (forward unreachable_code_transform ZL s ST a)) a
+    -> annotation s a
+    -> labelsDefined s (length ZL)
+    -> labelsDefined s (length BL)
+    -> paramsMatch s (length ⊝ ZL)
+    -> poLe (snd (@forward sT _ _ _ unreachable_code_transform ZL s ST a)) (Some ⊝ BL)
+    -> unreachable_code ZL BL s a.
+Proof.
+  intros EQ Ann DefZL DefBL PM.
+  general induction Ann; simpl in *; inv DefZL; inv DefBL; inv PM;
+    repeat let_case_eq; repeat simpl_pair_eqs; subst; simpl in *.
+  - inv EQ.
+    pose proof (ann_R_get H8); simpl in *.
+    econstructor.
+    eapply IHAnn; eauto;
+    simpl_forward_setTopAnn.
+  - assert (❬snd (forward unreachable_code_transform ZL s (subTerm_EQ_If1 eq_refl ST) sa)❭ =
+            ❬snd (forward unreachable_code_transform ZL t (subTerm_EQ_If2 eq_refl ST) ta)❭). {
+      eapply (@forward_length_ass _ (fun _ => bool)); eauto. symmetry.
+      eapply (@forward_length_ass _ (fun _ => bool)); eauto.
+    }
+    repeat cases in EQ; simpl in *; try solve [congruence]; inv EQ;
+    repeat simpl_forward_setTopAnn;
+    econstructor; intros; try solve [congruence];
+      eauto using PIR2_fstNoneOrR_inv_left, PIR2_fstNoneOrR_inv_right.
+  - inv_get.
+    edestruct (get_in_range _ H3) as [B ?]; eauto.
+    edestruct PIR2_nth; eauto using ListUpdateAt.list_update_at_get_3; dcr. inv_get.
+    destruct x1; isabsurd.
+    econstructor; eauto.
+  - econstructor.
+  - inv EQ.
+    pose proof (ann_R_get H8); simpl in *.
+    econstructor.
+    eapply IHAnn; eauto;
+    simpl_forward_setTopAnn.
+  - inv EQ.
+    econstructor; eauto.
+    + eapply IHAnn; eauto.
+
+    + intros.
+      edestruct (get_forwardF (fun _ => bool) (forward unreachable_code_transform)
+                              (fst ⊝ s ++ ZL) (subTerm_EQ_Fun2 eq_refl ST) H3 H4).
+      eapply H1; eauto. admit.
+    + intros.
+
+Qed.
+
+Definition livenessAnalysis s :=
+  let a := Analysis.safeFixpoint (LivenessAnalysis.liveness_analysis s) in
+  mapAnn (@proj1_sig _ _) (proj1_sig (proj1_sig a)).
+
+
+
+Ltac destr_sig H :=
+  match type of H with
+  | context [proj1_sig ?x] => destruct x; simpl in H
+  end.
+
+Tactic Notation "destr_sig" :=
+  match goal with
+  | [ |- context [proj1_sig (proj1_sig ?x)] ] => destruct x; simpl
+  | [ |- context [proj1_sig ?x] ] => destruct x; simpl
+  end.
+
+Definition correct s
+  : labelsDefined s 0
+    -> paramsMatch s nil
+    -> true_live_sound Imperative nil nil s (livenessAnalysis s).
+Proof.
+  intros.
+  unfold livenessAnalysis.
+  destr_sig. destr_sig. dcr.
+  eapply (@liveness_analysis_correct s nil nil s); eauto.
+  eapply H3.
+Qed.
